wip on an independent steel st spinlock implementation

pulse/ulib/experimental/Steel.ST.SpinLock.fst
@@ -15,9 +15,107 @@
 *)
 
 module Steel.ST.SpinLock
+
+open FStar.Ghost
+
+open Steel.ST.Effect
+open Steel.ST.Effect.Ghost
+open Steel.ST.Effect.Atomic
+
 open Steel.ST.Util
-open Steel.ST.Coercions
-module L = Steel.SpinLock
+open Steel.ST.Loops
+open Steel.ST.Reference
+
+let locked = true
+let unlocked = false
+
+[@@ __reduce__]
+let lockinv_predicate (p:vprop) (r:ref bool)
+  : bool -> vprop
+  = fun (b:bool) -> pts_to r full_perm b `star` (if b then emp else p)
+
+[@@ __reduce__]
+let lockinv (p:vprop) (r:ref bool) : vprop =
+  exists_ (lockinv_predicate p r)
+
+let lock_t = ref bool & erased iname
+let protects l p = snd l >--> lockinv p (fst l)
+
+assume //benign; this is defining admit__
+val admit__ (#a:Type)
+            (#p:pre_t)
+            (#q:a -> vprop)
+            (_:unit)
+  : STF a p q True (fun _ -> False)
+assume //benign; this is defining admit___
+val admit___ (#opened:_)
+             (#a:Type)
+             (#p:pre_t)
+             (#q:a -> vprop)
+             (_:unit)
+  : STAtomicF a opened p q True (fun _ -> False)
+
+let new_lock p =
+  let r = alloc unlocked in
+  rewrite (pts_to _ _ _ `star` p)
+          (lockinv_predicate p r unlocked);
+  intro_exists unlocked (lockinv_predicate p r);
+  let i = new_invariant (lockinv p r) in
+  return (r, i)
+
+[@@ __reduce__]
+let acquire_loop_inv (p:vprop) : bool -> vprop = fun b -> if b then emp else p
+
+[@@ __reduce__]
+let acquire_core (#opened:_) (p:vprop) (r:ref bool) ()
+  : STAtomicT bool opened
+      (lockinv p r `star` exists_ (acquire_loop_inv p))
+      (fun b -> lockinv p r `star` acquire_loop_inv p b)
+  = let w = elim_exists #_ #_ #(lockinv_predicate p r) () in
+    drop (exists_ _);
+    let b = cas r w unlocked locked in
+    if b
+    then begin
+      let res = false in
+      rewrite (if w then emp else p) p;
+      rewrite ((if b then _ else _) `star` emp)
+              (lockinv_predicate p r locked);
+      intro_exists locked (lockinv_predicate p r);
+      rewrite p (acquire_loop_inv p res);
+      return res
+    end
+    else begin
+      let res = true in
+      rewrite (if b then _ else _)
+              (pts_to r full_perm w);
+      intro_exists (Ghost.reveal w) (lockinv_predicate p r);
+      rewrite emp (acquire_loop_inv p res);
+      return res
+    end
+
+inline_for_extraction
+let acquire_loop_cond (p:vprop) (r:ref bool) (i:inv (lockinv p r)) ()
+  : STT bool (exists_ (acquire_loop_inv p))
+             (fun b -> acquire_loop_inv p b)
+  = with_invariant i (acquire_core p r)
+
+inline_for_extraction
+let acquire_loop_body (p:vprop) (r:ref bool) ()
+  : STT unit (acquire_loop_inv p true)
+             (fun _ -> exists_ (acquire_loop_inv p))
+  = intro_exists true (acquire_loop_inv p)
+
+let acquire #p l =
+  rewrite emp (acquire_loop_inv p true);
+  intro_exists true (acquire_loop_inv p);
+  while_loop
+    (acquire_loop_inv p)
+    (acquire_loop_cond p (fst l) (snd l))
+    (acquire_loop_body p (fst l));
+  rewrite (acquire_loop_inv p false) p
+
+let release #p l =
+
 
 let lock_t
   : Type u#0
